\documentclass[10pt]{article}

\usepackage{amsthm}
\usepackage{amsmath}
\usepackage{amsfonts}
\usepackage[margin=1in]{geometry}
\usepackage{titlesec}

\titleformat{\section}{\large\bfseries}
{\thesection}{0.5em}{}
\titleformat{\subsection}{\normalsize\itshape}
{\thesubsection}{0.5em}{}
\titlespacing*{\subsection}{0pt}{0pt}{0.1em}

\setlength{\parskip}{\baselineskip}
\setlength{\parindent}{0pt}

\title{Math 275A: Homework 7}
\author{Marcus Lucas}
\date{\vspace{-1cm}}


\begin{document}

\maketitle

\section*{3.2.1}

Define a collection of sets $A_{n,m_n}$ for $n \in \mathbb{N}^+$
and $m_n \in \{1,\dots,2^n\}$ where 
$A_{n,m_n} = (0,1) \setminus [\frac{m_n-1}{2^n}, \frac{m_n}{2^n}]$.
Define the collection of distributions $\mu_{n,m_n}$
to be uniform on each respective $A_{n,m_n}$
such that their corresponding distribution functions $F_{n,m_n}$
are have a constant positive slope, excepting the interval 
$(\frac{m_n-1}{2^n}, \frac{m_n}{2^n})$ where the slope is zero.
Let $F_1 = F_{1,1}, F_2 = F_{1,2}, F_3 = F_{2,1}, \dots$.
Then the sequence $F_k$ converges pointwise to $F$, 
the distribution function for the uniform distribution $\mu$.
And so $\mu_k \implies \mu$. 

At the same time, for any $x \in (0,1)$ there is an infinite
subcollection of density functions $f_k(x)$ which evaluate to
zero at $x$. Thus $f_k(x)$ does not converge to $f(x) = 1$
anywhere in $(0,1)$.


\section*{3.2.2.iii}
\textit{Claim:}
Let $X_1, X_2, \dots$ be independent with distribution $F$,
and let $M_n = \max_{m \le n}X_m$. Then $P(M_n \le x) = F(x)^n$.
Prove that if $F(x) = 1-e^{-x}$ for $x \ge 0$ then for all
$y \in (-\infty, \infty)$
\begin{equation*}
  P(M_n - \log n \le y) \to \exp(-e^-y)
\end{equation*}

\textit{Proof:}
First note that
\begin{equation*}
\begin{aligned}
  P(M_n - \log n \le y) &= P(M_n \le \log n + y) \\
  &= F(\log n + y)^n \\
  &= (1 - e^{-\log n - y})^n \\
  &= (1 - n^{-1}e^{-y})^n
\end{aligned}
\end{equation*}
We can apply Lemma 3.1.1 from Durrett to the last equation
(where $c_n = -n^{-1}e^{-y} \to 0$, $a_n = n \to \infty$,
and $c_n a_n = -e^{-y})$ to determine that
$P(M_n - \log n \le y) \to \exp(-e^{-y})$.

\section*{3.2.4}
\textit{Claim:}
Let $g \ge 0$ be continuous. If $X_n \implies X_\infty$ then
\begin{equation*}
  \underset{n \to \infty}{\lim \inf} \ E g(X_n) \ge E g(X_\infty)
\end{equation*}

\textit{Proof:}
We know from Fatou's lemma that, in general
\begin{equation*}
  \underset{n \to \infty}{\lim \inf} \ E g(X_n) 
  \ge E (\underset{n \to \infty}{\lim \inf} \ g(X_n)) 
\end{equation*}

\section*{3.2.10}

\section*{3.2.13}

\section*{Extra 1}

\end{document}